

MAP Estimate:

$$D = \{x_1, x_2, \dots, x_n\}$$

$$p_{\theta|D} = \frac{p_{D|\theta} p_{\theta}}{Z}$$

Consider estimating the mean of Gaussian density with variance assumed known.

$$p_{x|\mu} = \frac{1}{\sigma\sqrt{2\pi}} \exp\left\{-\frac{1}{2\sigma^2} (x-\mu)^2\right\}$$

μ is the only parameter.

$$\mu_{MLE} = \frac{1}{n} \sum_{i=1}^n x_i$$

$$p_{\mu|D} = \frac{p_{D|\mu} p_{\mu}}{Z}$$

* For conjugate prior, we want p_{μ} & $p_{\mu|D}$ to have the same funcⁿ form

$$p_{D|\mu} = \left(\frac{1}{\sigma\sqrt{2\pi}} \right)^n \exp \left\{ -\frac{1}{2\sigma^2} \sum_{i=1}^n (x_i - \mu)^2 \right\}$$

As a func of μ , this has an exponential of a quadratic in μ

* we need p_μ s.t., when multiplied by $p_{D|\mu}$ we need to get the same form as of p_μ

* \therefore the conjugate prior here is a normal density

* $p_\mu = \mathcal{N}(\mu_0, \sigma_0^2)$
where μ_0, σ_0^2 are hyper parameters.

$$p_{\mu|D} = \frac{p_{D|\mu} p_\mu}{Z}$$

$$\begin{aligned} p_{\mu|D} &\propto \exp \left\{ -\frac{1}{2\sigma^2} \sum_{i=1}^n (x_i - \mu)^2 - \frac{1}{2\sigma_0^2} (\mu - \mu_0)^2 \right\} \\ &= \exp \left\{ -\frac{1}{2} A \right\} \end{aligned}$$

$$A = \frac{1}{\sigma^2} \sum_{i=1}^n x_i^2 + \mu^2 \left(\frac{1}{\sigma_0^2} + \frac{n}{\sigma^2} \right) - 2\mu \left(\sum_{i=1}^n \frac{x_i}{\sigma^2} + \frac{\mu_0}{\sigma_0^2} \right) + \frac{\mu_0^2}{\sigma_0^2} \rightarrow \textcircled{1}$$

Suppose we have $\mu_{1|D}$ is $N(\mu_n, \sigma_n^2)$

$$\begin{aligned} \mu_{1|D} &\propto \exp \left\{ -\frac{1}{2} \frac{(\mu - \mu_n)^2}{\sigma_n^2} \right\} \\ &= \exp \left\{ -\frac{1}{2} \left[\frac{\mu^2}{\sigma_n^2} + \frac{\mu_n^2}{\sigma_n^2} - 2\mu \frac{\mu_n}{\sigma_n^2} \right] \right\} \\ &\quad \hookrightarrow \textcircled{2} \end{aligned}$$

now Comparing $\textcircled{1}$ & $\textcircled{2}$

$$\frac{1}{\sigma_n^2} = \frac{1}{\sigma_0^2} + \frac{n}{\sigma^2}$$

$$\sigma_n^2 = \frac{\sigma^2 \sigma_0^2}{\sigma^2 + n \sigma_0^2}$$

$$\frac{\mu_n}{\sigma_n^2} = \frac{1}{\sigma^2} \sum_{i=1}^n x_i + \frac{\mu_0}{\sigma_0^2}$$

$$\mu_n = \frac{\sigma_n^2}{\sigma^2} \sum_{i=1}^n x_i + \frac{\sigma_n^2}{\sigma_0^2} \mu_0$$

μ_n is a convex combⁿ of MLE & μ_0

* for large n $\mu_n \approx \mu_{MLE}$

As n becomes very large Bayesian Estimate is same as MLE

* Since the distribution is Gaussian

mode as well as mean is μ_n